CellularAutomatas/proofs/lcellautomaton.lean
@@ -1,0 +1,186 @@
+import CellularAutomatas.defs
+import CellularAutomatas.proofs.find_some
+
+@[simp]
+lemma nextt0 (C: CellAutomaton) (c: Config C.Q): C.nextt c 0 = c := by simp [CellAutomaton.nextt, apply_iterated]
+
+@[simp]
+lemma nextt1 (C: CellAutomaton) (c: Config C.Q): C.nextt c 1 = C.next c := by simp [CellAutomaton.nextt, apply_iterated]
+
+
+@[simp]
+lemma LCellAutomaton.comp_zero {C: LCellAutomaton α} {w}: C.comp w 0 = C.embed_word w := by rfl
+
+lemma LCellAutomaton.embed_word_eq (C: LCellAutomaton α) {w: Word α} {p: ℤ} (h: p ∈ w.range):
+    C.embed_word w p = C.embed (w.get' p h) := by
+      grind [LCellAutomaton.embed_word, Word.get']
+
+lemma LCellAutomaton.nextt_succ_eq (C: LCellAutomaton α) (c: Config C.Q): C.nextt c (t + 1) = C.next (C.nextt c t) := by
+  simp [CellAutomaton.nextt, apply_iterated_succ_apply']
+
+
+
+lemma LCellAutomaton.comp_succ_eq (C: LCellAutomaton α): C.comp w (t + 1) = C.next (C.comp w t) := by
+  funext i
+  simp [LCellAutomaton.comp, LCellAutomaton.nextt_succ_eq]
+
+
+
+lemma δδt_succ {C: CellAutomaton} {q: C.Q} {t: ℕ} : δδt q (t + 1) = δδ (δδt q t) := by
+  simp [δδt, apply_iterated_succ_apply']
+
+@[simp]
+lemma δδt_zero {C: CellAutomaton} {q: C.Q} : δδt q 0 = q := by
+  simp [δδt]
+
+lemma CellAutomaton.δδ_of_quiescent {C: CellAutomaton} {q: C.Q} (h: C.quiescent q): δδ q = q := by
+  simp_all [δδ, CellAutomaton.quiescent, CellAutomaton.quiescent_set]
+
+lemma CellAutomaton.δ_of_quiescent {C: CellAutomaton} {q: C.Q} (h: C.quiescent q): C.δ q q q = q := by
+  simp_all [CellAutomaton.quiescent, CellAutomaton.quiescent_set]
+
+lemma CellAutomaton.δδ_of_quiescent2 {C: CellAutomaton} {q: C.Q} (h: C.quiescent q): δδ q = q := by
+  simp_all [δδ, CellAutomaton.δ_of_quiescent]
+
+lemma CellAutomaton.delta_of_dead {C: CellAutomaton} {b: C.Q} (h: C.dead b) (a c: C.Q): C.δ a b c = b := by
+  simp_all [CellAutomaton.dead, CellAutomaton.delta_closed_set]
+
+
+
+lemma CellAutomaton.next_state_of_closed_set_state
+  {C: CellAutomaton} {S} {c: Config C.Q} {i} (h1: C.delta_closed_set S) (h2: c i ∈ S):
+    C.next c i ∈ S := by
+  unfold CellAutomaton.next
+  unfold CellAutomaton.delta_closed_set at h1
+  exact h1 (c (i - 1)) ⟨c i, h2⟩ (c (i + 1))
+
+
+lemma CellAutomaton.quiescent_of_dead {C: CellAutomaton} {q: C.Q} (h: C.dead q): C.quiescent q := by
+  unfold CellAutomaton.quiescent
+  intro a b c
+  unfold CellAutomaton.dead at h
+  unfold CellAutomaton.delta_closed_set at h
+  simp_all only [Set.mem_singleton_iff, Subtype.forall, forall_eq]
+  obtain ⟨a, a_h⟩ := a
+  obtain ⟨b, b_h⟩ := b
+  obtain ⟨c, c_h⟩ := c
+  simp_all only
+  simp_all only [Set.mem_singleton_iff]
+
+
+
+def uniform_config {C: CellAutomaton} (q: C.Q): Config C.Q := fun _ => q
+
+@[simp]
+lemma uniform_config_at_eq {C: CellAutomaton} (q: C.Q) (i: ℤ): uniform_config q i = q := by rfl
+
+
+
+
+
+
+
+
+@[simp]
+lemma empty_word_range: @Word.range α [] = {} := by
+  unfold Word.range
+  ext x
+  simp_all
+
+
+
+def Word.cone (w: Word α) (t: ℕ): Set ℤ := { i: ℤ | -t ≤ i ∧ i < w.length + t }
+
+instance (w: Word α) (t: ℕ) (i: ℤ) [d: Decidable (i ∈ { i: ℤ | -t ≤ i ∧ i < w.length + t })]:
+  Decidable (i ∈ (Word.cone w t)) := d
+
+section
+  variable {w: Word α}
+
+  lemma Word.cone_prop {t: ℕ} {i: ℤ} (d: ℤ) (h: i ∉ w.cone (t + 1)) (h2: d.natAbs ≤ 1): (i + d) ∉ w.cone t := by
+    simp_all [Word.cone]
+    omega
+
+  lemma Word.cone_prop' {t: ℕ} {i: ℤ} { d: ℤ } (h: (i + d) ∈ w.cone t) (h2: d.natAbs ≤ 1): i ∈ w.cone (t + 1) := by
+    simp_all [Word.cone]
+    omega
+
+  lemma Word.cone_prop'' {t: ℕ} {i: ℤ} (h: i ∈ w.cone t): i ∈ w.cone (t + 1) := by
+    simp_all [Word.cone]
+    omega
+
+
+  lemma Word.cone_succ {t: ℕ} {i: ℤ} (h1: i - 1 ∈ w.cone t) (h2: i + 1 ∈ w.cone t): i ∈ w.cone (t + 1) := by
+    simp_all [Word.cone]
+    omega
+
+  lemma Word.cone_succ_not {t: ℕ} {i: ℤ} (wlen: w.length > 0) (h1: i - 1 ∉ w.cone t) (h2: i ∉ w.cone t) (h3: i + 1 ∉ w.cone t): i ∉ w.cone (t + 1) := by
+    simp_all [cone]
+    omega
+
+  @[simp]
+  lemma Word.cone_zero_eq_range: w.cone 0 = w.range := by simp [Word.cone, Word.range]
+
+  def Word.get_cone_0 {i} (h: i ∈ w.cone 0) := w.get' i (Word.cone_zero_eq_range ▸ h)
+
+  lemma Word.zero_mem_cone (h: w.length > 0) (t): 0 ∈ w.cone t := by
+    simp [Word.cone]
+    omega
+end
+
+
+
+section
+  variable {C: LCellAutomaton α}
+  variable {w: Word α}
+
+
+
+  lemma LCellAutomaton.empty_word_config_eq_uniform_border: C.embed_word [] = uniform_config C.border := by
+    funext i
+    simp [LCellAutomaton.embed_word, uniform_config, uniform_config]
+
+
+
+  lemma LCellAutomaton.uniform_state_eq {q: C.Q}: C.nextt (uniform_config q) = uniform_config ∘ (δδt q) := by
+    funext t i
+    simp only [CellAutomaton.nextt, δδt, Function.comp_apply, uniform_config]
+
+    induction t generalizing i
+    case h.h.zero =>
+      simp [uniform_config, apply_iterated_zero]
+    case h.h.succ n ih =>
+      simp [apply_iterated_succ_apply', ih, δδ, CellAutomaton.next]
+
+  lemma LCellAutomaton.comp_empty_eq_uniform: C.comp [] = uniform_config ∘ (δδt C.border) := by
+    simp [LCellAutomaton.comp, LCellAutomaton.empty_word_config_eq_uniform_border, LCellAutomaton.uniform_state_eq]
+
+
+
+  lemma LCellAutomaton.embed_word_eq_embed {i} (h: i ∈ w.cone 0): C.embed_word w i = C.embed (w.get_cone_0 h) := by
+    rw [Word.cone_zero_eq_range] at h
+    simp_all [LCellAutomaton.embed_word, Word.get_cone_0]
+
+
+
+
+
+
+  lemma LCellAutomaton.comp_outside_word_cone_eq_border_pow_t {t: ℕ} {i: ℤ} (h: i ∉ w.cone t):
+      C.comp w t i = δδt C.border t := by
+
+    induction t generalizing i
+    case zero =>
+      simp_all [LCellAutomaton.comp, CellAutomaton.nextt, δδt, LCellAutomaton.embed_word, Word.cone_zero_eq_range]
+    case succ t ih =>
+      have h1 := ih $ Word.cone_prop 0 h (by simp)
+      have h2 := ih $ Word.cone_prop (-1) h (by simp)
+      have h3 := ih $ Word.cone_prop 1 h (by simp)
+      have x: (i + -1) = i - 1 := by rfl
+
+      rw [LCellAutomaton.comp_succ_eq]
+      rw [δδt_succ]
+      set c := C.comp w t
+      simp_all [CellAutomaton.next, δδ]
+
+end
